theories/zoo_parabs/vertex.v
@@ -169,32 +169,67 @@ Module base.
     #[local] Instance : CustomIpat "finished" :=
       "#Hstate{which;}₁{_{}}".
 
-    Definition vertex_wp t γ P R task iter : iProp Σ :=
+    Definition vertex_wp_body t γ P R wp task iter : iProp Σ :=
       ∀ pool ctx scope iter',
       pool_context pool ctx scope -∗
       vertex_ready iter -∗
       vertex_model t γ task iter' -∗
       WP task ctx {{ res,
-        ∃ task,
-        ⌜res = ()%V⌝ ∗
+        ∃ b task,
+        ⌜res = #b⌝ ∗
         pool_context pool ctx scope ∗
         vertex_model t γ task iter' ∗
-        ▷ P ∗
-        ▷ □ R
+        if b then
+          ▷ P ∗
+          ▷ □ R
+        else
+          ▷ wp task iter'
       }}.
+    #[local] Definition vertex_wp_pre
+    : location → vertex_name → iProp Σ → iProp Σ →
+      (val -d> vertex_iteration -d> iProp Σ) →
+      val -d> vertex_iteration -d> iProp Σ
+    :=
+      vertex_wp_body.
+    #[local] Instance vertex_wp_pre_contractive t γ P R :
+      Contractive (vertex_wp_pre t γ P R).
+    Proof.
+      rewrite /vertex_wp_pre /vertex_wp_body.
+      solve_contractive.
+    Qed.
+    #[local] Instance vertex_wp_pre_ne t γ P R :
+      NonExpansive (vertex_wp_pre t γ P R).
+    Proof.
+      apply _.
+    Qed.
+    Definition vertex_wp t γ P R : val → vertex_iteration → iProp Σ :=
+      fixpoint (vertex_wp_pre t γ P R).
 
+    Lemma vertex_wp_unfold t γ P R task iter :
+      vertex_wp t γ P R task iter ⊣⊢
+      vertex_wp_body t γ P R (vertex_wp t γ P R) task iter.
+    Proof.
+      apply (fixpoint_unfold (vertex_wp_pre t γ P R)).
+    Qed.
     #[global] Instance vertex_wp_ne n :
       Proper (
         (=) ==>
         (=) ==>
         (≡{n}≡) ==>
         (≡{n}≡) ==>
-        (=) ==>
-        (=) ==>
+        (≡{n}≡) ==>
+        (≡{n}≡) ==>
         (≡{n}≡)
       ) vertex_wp.
     Proof.
-      solve_proper.
+      intros t t_ <- γ γ_ <-.
+      induction (lt_wf n) as [n _ IH] => P1 P2 HP R1 R2 HR task task_ <- iter iter_ <-.
+      rewrite !vertex_wp_unfold /vertex_wp_body.
+      do 21 f_equiv. 1: solve_proper.
+      f_contractive.
+      apply (dist_le _ m) in HP; last by apply SIdx.lt_le_incl.
+      apply (dist_le _ m) in HR; last by apply SIdx.lt_le_incl.
+      apply IH; done.
     Qed.
 
     #[local] Definition inv_state_init preds iter Π : iProp Σ :=
@@ -689,7 +724,7 @@ Module base.
         RET #t;
         meta_token t ⊤ ∗
         vertex_inv t γ P R ∗
-        vertex_model t γ (default (fun: <> => ())%V task) iter ∗
+        vertex_model t γ (default (fun: <> => true)%V task) iter ∗
         vertex_output γ P
       }}}.
     Proof.
@@ -699,7 +734,7 @@ Module base.
 
       wp_bind (Match _ _ _ _).
       wp_apply (wp_wand (λ res,
-        ⌜res = default (fun: <> => ())%V task⌝
+        ⌜res = default (fun: <> => true)%V task⌝
       )%I) as (res) "->".
       { destruct task; iSteps. }
 
@@ -729,6 +764,26 @@ Module base.
       - rewrite /inv_state /inv_state_init.
         iExists ∅. rewrite big_sepMS_empty left_id. iSteps.
       - iExists []. iSteps.
+    Qed.
+
+    Lemma vertex_create'_spec P R task :
+      {{{
+        True
+      }}}
+        vertex_create' task
+      {{{ t γ iter,
+        RET #t;
+        meta_token t ⊤ ∗
+        vertex_inv t γ P R ∗
+        vertex_model t γ (fun: "ctx" => task "ctx" ;; true) iter ∗
+        vertex_output γ P
+      }}}.
+    Proof.
+      iIntros "%Φ _ HΦ".
+
+      wp_rec.
+      wp_smart_apply (vertex_create_spec P R (Some _) with "[//]").
+      iSteps.
     Qed.
 
     Lemma vertex_task_spec t γ task iter :
@@ -1046,27 +1101,36 @@ Module base.
         iIntros "{%} !>".
 
         wp_load.
-        wp_apply (wp_wand with "(Htask Hctx [$] [$])") as (res) "{%} (%task & -> & Hctx & (:model) & HP & #HR)".
-        wp_load.
 
-        awp_apply (mpmc_stack_2_close_spec with "Hsuccessors_inv") without "Hctx".
-        iInv "Hinv" as "(:inv_inner =2)".
-        iDestruct (state_agree with "Hstate₁ Hstate₂") as %<-.
-        iDestruct "Hinv_state" as "(:inv_state_init =2 >)".
-        iDestruct "Hinv_successors" as "(:inv_successors =2)".
-        iAaccIntro with "Hsuccessors_model"; iIntros "Hsuccessors_model"; first iFrameSteps.
-        iMod (state_update Finished with "Hstate₁ Hstate₂") as "(Hstate₁ & Hstate₂)".
-        iMod (state₁_discard with "Hstate₁") as "#Hstate₁".
-        iDestruct (output_produce with "Houtput_auth HP") as "Houtput_auth".
-        iSplitR "Hsuccs". { iFrameSteps. }
-        iIntros "!> H£ Hctx {%}".
+        rewrite vertex_wp_unfold.
+        wp_apply (wp_wand with "(Htask Hctx [$] [$])") as (res) "{%} (%b & %task & -> & Hctx & (:model) & Hb)".
+        destruct b.
 
-        iMod (lc_fupd_elim_later with "H£ Hsuccs") as "Hsuccs".
-        wp_smart_apply (clst_iter_spec (λ _, pool_context pool ctx scope) with "[$Hctx Hsuccs]"); [done | | iSteps].
-        rewrite big_sepL_fmap.
-        iApply (big_sepL_impl with "Hsuccs"). iIntros "!> %i %succ _ (:inv_successor) Hctx".
-        wp_smart_apply ("IHrelease_successor" with "[$Hctx $Hpredecessors_elem $Hstate₁]"); last iSteps.
-        iApply (vertex_inv_unfold with "Hinv_succ").
+        - iDestruct "Hb" as "(HP & #HR)".
+
+          wp_load.
+
+          awp_apply (mpmc_stack_2_close_spec with "Hsuccessors_inv") without "Hctx".
+          iInv "Hinv" as "(:inv_inner =2)".
+          iDestruct (state_agree with "Hstate₁ Hstate₂") as %<-.
+          iDestruct "Hinv_state" as "(:inv_state_init =2 >)".
+          iDestruct "Hinv_successors" as "(:inv_successors =2)".
+          iAaccIntro with "Hsuccessors_model"; iIntros "Hsuccessors_model"; first iFrameSteps.
+          iMod (state_update Finished with "Hstate₁ Hstate₂") as "(Hstate₁ & Hstate₂)".
+          iMod (state₁_discard with "Hstate₁") as "#Hstate₁".
+          iDestruct (output_produce with "Houtput_auth HP") as "Houtput_auth".
+          iSplitR "Hsuccs". { iFrameSteps. }
+          iIntros "!> H£ Hctx {%}".
+
+          iMod (lc_fupd_elim_later with "H£ Hsuccs") as "Hsuccs".
+          wp_smart_apply (clst_iter_spec (λ _, pool_context pool ctx scope) with "[$Hctx Hsuccs]"); [done | | iSteps].
+          rewrite big_sepL_fmap.
+          iApply (big_sepL_impl with "Hsuccs"). iIntros "!> %i %succ _ (:inv_successor) Hctx".
+          wp_smart_apply ("IHrelease_successor" with "[$Hctx $Hpredecessors_elem $Hstate₁]"); last iSteps.
+          iApply (vertex_inv_unfold with "Hinv_succ").
+
+        - wp_smart_apply ("IHrelease" with "[$]").
+          iSteps.
       }
     Qed.
     Lemma vertex_release_spec pool ctx scope t γ P R task iter :
@@ -1086,24 +1150,21 @@ Module base.
       iApply "H".
     Qed.
 
-    Lemma vertex_yield_spec pool ctx scope t γ P R task' iter task :
+    Lemma vertex_yield_spec t γ task' iter task :
       {{{
-        pool_context pool ctx scope ∗
-        vertex_inv t γ P R ∗
-        vertex_model t γ task' iter ∗
-        vertex_wp t γ P R task iter
+        vertex_model t γ task' iter
       }}}
-        vertex_yield ctx #t task
+        vertex_yield #t task
       {{{
-        RET ();
-        pool_context pool ctx scope
+        RET false;
+        vertex_model t γ task iter
       }}}.
     Proof.
-      iIntros "%Φ (Hctx & #Hinv & Hmodel & Htask) HΦ".
+      iIntros "%Φ Hmodel HΦ".
 
       wp_rec.
       wp_smart_apply (vertex_set_task_spec with "[$]") as "Hmodel".
-      wp_smart_apply (vertex_release_spec with "[$] HΦ").
+      iSteps.
     Qed.
   End vertex_G.
 
@@ -1215,44 +1276,82 @@ Section vertex_G.
       )
     ".
 
-  Definition vertex_wp t P R task iter : iProp Σ :=
+  Definition vertex_wp_body t P R wp task iter : iProp Σ :=
     ∀ pool ctx scope iter',
     pool_context pool ctx scope -∗
     vertex_ready iter -∗
     vertex_model t task iter' -∗
     WP task ctx {{ res,
-      ∃ task,
-      ⌜res = ()%V⌝ ∗
+      ∃ b task,
+      ⌜res = #b⌝ ∗
       pool_context pool ctx scope ∗
       vertex_model t task iter' ∗
-      ▷ P ∗
-      ▷ □ R
+      if b then
+        ▷ P ∗
+        ▷ □ R
+      else
+        ▷ wp task iter'
     }}.
+  #[local] Definition vertex_wp_pre
+  : val → iProp Σ → iProp Σ →
+    (val -d> vertex_iteration -d> iProp Σ) →
+    val -d> vertex_iteration -d> iProp Σ
+  :=
+    vertex_wp_body.
+  #[local] Instance vertex_wp_pre_contractive t P R :
+    Contractive (vertex_wp_pre t P R).
+  Proof.
+    rewrite /vertex_wp_pre /vertex_wp_body.
+    solve_contractive.
+  Qed.
+  #[local] Instance vertex_wp_pre_ne t P R :
+    NonExpansive (vertex_wp_pre t P R).
+  Proof.
+    apply _.
+  Qed.
+  Definition vertex_wp t P R : val → vertex_iteration → iProp Σ :=
+    fixpoint (vertex_wp_pre t P R).
 
+  Lemma vertex_wp_unfold t P R task iter :
+    vertex_wp t P R task iter ⊣⊢
+    vertex_wp_body t P R (vertex_wp t P R) task iter.
+  Proof.
+    apply (fixpoint_unfold (vertex_wp_pre t P R)).
+  Qed.
   #[global] Instance vertex_wp_ne n :
     Proper (
       (=) ==>
       (≡{n}≡) ==>
       (≡{n}≡) ==>
-      (=) ==>
-      (=) ==>
+      (≡{n}≡) ==>
+      (≡{n}≡) ==>
       (≡{n}≡)
     ) vertex_wp.
   Proof.
-    solve_proper.
+    intros t t_ <-.
+    induction (lt_wf n) as [n _ IH] => P1 P2 HP R1 R2 HR task task_ <- iter iter_ <-.
+    rewrite !vertex_wp_unfold /vertex_wp_body.
+    do 21 f_equiv. 1: solve_proper.
+    f_contractive.
+    apply (dist_le _ m) in HP; last by apply SIdx.lt_le_incl.
+    apply (dist_le _ m) in HR; last by apply SIdx.lt_le_incl.
+    apply IH; done.
   Qed.
-  #[local] Lemma vertex_wp_to_raw 𝑡 γ P R task iter :
+  #[local] Lemma vertex_wp_to_base 𝑡 γ P R task iter :
     meta 𝑡 nroot γ -∗
     vertex_wp #𝑡 P R task iter -∗
     base.vertex_wp 𝑡 γ P R task iter.
   Proof.
+    iLöb as "HLöb" forall (task iter).
+
+    iEval (rewrite vertex_wp_unfold base.vertex_wp_unfold).
     iIntros "#Hmeta Hwp %pool %ctx %scope %iter' Hctx Hready Hmodel".
 
-    wp_apply (wp_wand with "(Hwp Hctx Hready [$Hmodel])") as (res) "{%} (%task & -> & ($ & Hmodel & $ & $))"; first iSteps.
-    iExists task. iSteps.
+    wp_apply (wp_wand with "(Hwp Hctx Hready [$Hmodel])") as (res) "{%} (%b & %task & -> & ($ & Hmodel & Hwp))"; first iSteps.
+    iExists b, task. iStep.
     iDestruct "Hmodel" as "(:model =1)". simplify.
     iDestruct (meta_agree with "Hmeta Hmeta_1") as %<-. iClear "Hmeta_1".
-    iFrame.
+    destruct b; iFrameSteps.
   Qed.
 
   #[global] Instance vertex_output_contractive t :
@@ -1421,7 +1520,7 @@ Section vertex_G.
     {{{ t iter,
       RET t;
       vertex_inv t P R ∗
-      vertex_model t (default (fun: <> => ())%V task) iter ∗
+      vertex_model t (default (fun: <> => true)%V task) iter ∗
       vertex_output t P
     }}}.
   Proof.
@@ -1429,6 +1528,26 @@ Section vertex_G.
 
     iApply wp_fupd.
     wp_apply (base.vertex_create_spec with "[//]") as (𝑡 γ iter) "(Hmeta & #Hinv & Hmodel & Houtput)".
+    iMod (meta_set with "Hmeta") as "#Hmeta"; first done.
+    iSteps.
+  Qed.
+
+  Lemma vertex_create'_spec P R task :
+    {{{
+      True
+    }}}
+      vertex_create' task
+    {{{ t iter,
+      RET t;
+      vertex_inv t P R ∗
+      vertex_model t (fun: "ctx" => task "ctx" ;; true) iter ∗
+      vertex_output t P
+    }}}.
+  Proof.
+    iIntros "%Φ _ HΦ".
+
+    iApply wp_fupd.
+    wp_apply (base.vertex_create'_spec with "[//]") as (𝑡 γ iter) "(Hmeta & #Hinv & Hmodel & Houtput)".
     iMod (meta_set with "Hmeta") as "#Hmeta"; first done.
     iSteps.
   Qed.
@@ -1502,29 +1621,52 @@ Section vertex_G.
   Proof.
     iIntros "%Φ (Hctx & (:inv =1) & (:model =2) & Htask) HΦ". simplify.
     iDestruct (meta_agree with "Hmeta_1 Hmeta_2") as %<-. iClear "Hmeta_2".
-    iDestruct (vertex_wp_to_raw with "Hmeta_1 Htask") as "Htask".
+    iDestruct (vertex_wp_to_base with "Hmeta_1 Htask") as "Htask".
 
     wp_apply (base.vertex_release_spec with "[$] HΦ").
   Qed.
-
-  Lemma vertex_yield_spec pool ctx scope t γ P R task' iter task :
+  Lemma vertex_release_spec' pool ctx scope t P R task iter :
     {{{
       pool_context pool ctx scope ∗
       vertex_inv t P R ∗
-      vertex_model t task' iter ∗
-      vertex_wp t P R task iter
+      vertex_model t task iter ∗
+      ( ∀ pool ctx scope,
+        pool_context pool ctx scope -∗
+        vertex_ready iter -∗
+        WP task ctx {{ res,
+          ⌜res = true%V⌝ ∗
+          pool_context pool ctx scope ∗
+          ▷ P ∗
+          ▷ □ R
+        }}
+      )
     }}}
-      vertex_yield ctx t task
+      vertex_release ctx t
     {{{
       RET ();
       pool_context pool ctx scope
     }}}.
   Proof.
-    iIntros "%Φ (Hctx & (:inv =1) & (:model =2) & Htask) HΦ". simplify.
-    iDestruct (meta_agree with "Hmeta_1 Hmeta_2") as %<-. iClear "Hmeta_2".
-    iDestruct (vertex_wp_to_raw with "Hmeta_1 Htask") as "Htask".
+    iIntros "%Φ (Hctx & #Hinv & Hmodel & Htask) HΦ".
 
-    wp_apply (base.vertex_yield_spec with "[$] HΦ").
+    wp_apply (vertex_release_spec with "[- HΦ] HΦ").
+    rewrite vertex_wp_unfold. iFrame "#∗". iSteps.
+  Qed.
+
+  Lemma vertex_yield_spec t task' iter task :
+    {{{
+      vertex_model t task' iter
+    }}}
+      vertex_yield t task
+    {{{
+      RET false;
+      vertex_model t task iter
+    }}}.
+  Proof.
+    iIntros "%Φ (:model) HΦ".
+
+    wp_apply (base.vertex_yield_spec with "[$]").
+    iSteps.
   Qed.
 End vertex_G.
 
