theories/examples/vertex_simple.v
@@ -59,26 +59,22 @@ Section vertex_simple_G.
     wp_rec.
     wp_smart_apply (mpsc_flag_create_spec P_d with "[//]") as (flag) "(#Hflag_inv & Hflag_consumer)".
 
-    wp_smart_apply (vertex_create_spec
+    wp_smart_apply (vertex_create'_spec
       (P_ab ∗ P_ac)
       True
-      (Some _)
     with "[//]") as (vtx_a iter_a) "(#Hvtx_a_inv & Hvtx_a_model & Hvtx_a_output)".
     iMod (vertex_output_split with "Hvtx_a_inv Hvtx_a_output") as "(Hvtx_a_output_b & Hvtx_a_output_c)".
-    wp_smart_apply (vertex_create_spec
+    wp_smart_apply (vertex_create'_spec
       P_b
       True
-      (Some _)
     with "[//]") as (vtx_b iter_b) "(#Hvtx_b_inv & Hvtx_b_model & Hvtx_b_output)".
-    wp_smart_apply (vertex_create_spec
+    wp_smart_apply (vertex_create'_spec
       P_c
       True
-      (Some _)
     with "[//]") as (vtx_c iter_c) "(#Hvtx_c_inv & Hvtx_c_model & Hvtx_c_output)".
-    wp_smart_apply (vertex_create_spec
+    wp_smart_apply (vertex_create'_spec
       True
       True
-      (Some _)
     with "[//]") as (vtx_d iter_d) "(#Hvtx_d_inv & Hvtx_d_model & _)".
 
     wp_smart_apply (vertex_precede_spec with "[$Hvtx_b_model]") as "(Hvtx_b_model & #Hvtx_a_predecessor_b)". 1: iFrame "#".
@@ -93,42 +89,54 @@ Section vertex_simple_G.
     )%I with "[- HΦ $Hpool_model]") as (?) "(Hpool_model & HP_d)".
     { iIntros "%ctx %scope Hctx".
 
-      wp_smart_apply (vertex_release_spec with "[$Hctx $Hvtx_d_model Hvtx_b_output Hvtx_c_output Hd]") as "Hctx".
-      { iFrame "#". iIntros "{%} %pool %ctx %scope %iter_d' Hctx Hvtx_d_ready Hvtx_d_model".
+      wp_smart_apply (vertex_release_spec' with "[$Hctx $Hvtx_d_model Hvtx_b_output Hvtx_c_output Hd]") as "Hctx".
+      { iFrame "#". iIntros "{%} %pool %ctx %scope Hctx #Hvtx_d_ready".
+
         wp_pures credits:"H£".
         iDestruct (lc_weaken 2 with "H£") as "H£". 1: done.
+
         iDestruct (vertex_predecessor_finished with "Hvtx_b_predecessor Hvtx_d_ready") as "#Hvtx_b_finished".
         iMod (vertex_inv_finished_output with "Hvtx_b_inv Hvtx_b_finished Hvtx_b_output") as "HP_b".
+
         iDestruct (vertex_predecessor_finished with "Hvtx_c_predecessor Hvtx_d_ready") as "#Hvtx_c_finished".
         iMod (vertex_inv_finished_output with "Hvtx_c_inv Hvtx_c_finished Hvtx_c_output") as "HP_c".
+
         iMod (lc_fupd_elim_laterN _ (P_b ∗ P_c) with "H£ [$]") as "(HP_b & HP_c)".
         wp_apply (wp_wand with "(Hd HP_b HP_c)") as (res) "(-> & HP_d)".
+
         wp_smart_apply (mpsc_flag_set_spec with "[$Hflag_inv $HP_d]").
         iSteps => //.
       }
 
-      wp_smart_apply (vertex_release_spec with "[$Hctx $Hvtx_c_model Hvtx_a_output_c Hc]") as "Hctx".
-      { iFrame "#". iIntros "{%} %pool %ctx %scope %iter_c' Hctx Hvtx_c_ready Hvtx_c_model".
+      wp_smart_apply (vertex_release_spec' with "[$Hctx $Hvtx_c_model Hvtx_a_output_c Hc]") as "Hctx".
+      { iFrame "#". iIntros "{%} %pool %ctx %scope Hctx #Hvtx_c_ready".
+
         wp_pures credits:"H£".
         iDestruct (lc_weaken 2 with "H£") as "H£". 1: done.
+
         iDestruct (vertex_predecessor_finished with "Hvtx_a_predecessor_c Hvtx_c_ready") as "#Hvtx_a_finished".
         iMod (vertex_inv_finished_output' with "H£ Hvtx_a_inv Hvtx_a_finished Hvtx_a_output_c") as "HP_ac".
+
         wp_apply (wp_wand with "(Hc HP_ac)") as (res) "(-> & $)".
         iSteps => //.
       }
 
-      wp_smart_apply (vertex_release_spec with "[$Hctx $Hvtx_b_model Hvtx_a_output_b Hb]") as "Hctx".
-      { iFrame "#". iIntros "{%} %pool %ctx %scope %iter_b' Hctx Hvtx_b_ready Hvtx_b_model".
+      wp_smart_apply (vertex_release_spec' with "[$Hctx $Hvtx_b_model Hvtx_a_output_b Hb]") as "Hctx".
+      { iFrame "#". iIntros "{%} %pool %ctx %scope Hctx #Hvtx_b_ready".
+
         wp_pures credits:"H£".
         iDestruct (lc_weaken 2 with "H£") as "H£". 1: done.
+
         iDestruct (vertex_predecessor_finished with "Hvtx_a_predecessor_b Hvtx_b_ready") as "#Hvtx_a_finished".
         iMod (vertex_inv_finished_output' with "H£ Hvtx_a_inv Hvtx_a_finished Hvtx_a_output_b") as "HP_ab".
+
         wp_apply (wp_wand with "(Hb HP_ab)") as (res) "(-> & $)".
         iSteps => //.
       }
 
-      wp_smart_apply (vertex_release_spec with "[$Hctx $Hvtx_a_model Ha]") as "Hctx".
-      { iFrame "#". iIntros "{%} %pool %ctx %scope %iter_a' Hctx Hvtx_a_ready Hvtx_a_model".
+      wp_smart_apply (vertex_release_spec' with "[$Hctx $Hvtx_a_model Ha]") as "Hctx".
+      { iFrame "#". iIntros "{%} %pool %ctx %scope Hctx Hvtx_a_ready".
+
         wp_smart_apply (wp_wand with "Ha") as (res) "(-> & $)".
         iSteps => //.
       }
